src/syntax.lean
@@ -5,70 +5,90 @@ import util
 
 variable {α : Type}
 
-/- Each program has names. Names consist of a finite set of class names. To each class name, there an associated finite set of field and method names. To each method name, there is an associated finite set of parameter names. -/
+/- Each program has names. Names consist of a finite set of class names, and a finite set of record names, which are disjoint. To each class name, there an associated finite set of field and method names. To each method name, there is an associated finite set of parameter names. There is a built-in record name, bool. -/
 class names (α : Type) :=
   (decidable_name: decidable_eq α)
   (Nc: finset α)
+  (Nr: finset α)
+  (Ndisjoint: disjoint Nc Nr)
   (Nf {x : α} (H: x ∈ Nc): finset α)
   (Nm {x : α} (H: x ∈ Nc): finset α)
   (Np {x : α} {H: x ∈ Nc} {y : α} (G : y ∈ Nm H): finset α)
+  (Nboolean : α)
+  (Hboolean : Nboolean ∈ Nr)
 instance names.decidable [names α]:
   decidable_eq α := names.decidable_name α
 
-section -- (scope: [names α], self, m)
-  variable [names α]
-  /- We make use of subtypes, to demonstrate instances of fintype. Whenever we have established that these types are finite, we obtain decidable equality for functions that take these types as domain (thanks to Johannes Hölzl). This fact turns out to be crucial for semantics. -/
-  @[reducible]
-  def class_name (α : Type) [names α] :=
-    {name : α // name ∈ names.Nc α}
-  variable {self : class_name α}
-  @[reducible]
-  def field_name (self : class_name α) :=
-    {name : α // name ∈ names.Nf self.property}
-  @[reducible]
-  def method_name (self : class_name α) :=
-    {name : α // name ∈ names.Nm self.property}
-  @[reducible]
-  def param_name (m : method_name self) :=
-    {name : α // name ∈ names.Np m.property}
-  /- A type in our object language is either: a reference type (by class name), or a data type from the host language. A variable context is a list of types; a local variable is encoded by an index in this context. Local variables do not have a name. -/
-  structure datatype :=
-    (host : Type)
-    (default: host)
-    (decidable_data: decidable_eq host)
-  instance datatype.to_sort : has_coe_to_sort datatype :=
-    {S := Type, coe := λS, S.host}
-  instance datatype.host_decidable (γ : datatype) :
-    decidable_eq γ := γ.decidable_data
-  instance datatype.host_inhabited (γ : datatype) :
-    inhabited γ := ⟨γ.default⟩
-  inductive type (α : Type) [names α]
-  | ref: class_name α → type
-  | data: datatype → type
-  @[reducible] def boolean (α : Type) [names α] : type α :=
-    type.data α ⟨bool, ff, bool.decidable_eq⟩
-  /- A local variable context is a list of types. -/
-  @[reducible] def context (α : Type) [names α] := list (type α)
+/- We make use of subtypes, to demonstrate instances of fintype. Whenever we have established that these types are finite, we obtain decidable equality for functions that take these types as domain (thanks to Johannes Hölzl). This fact turns out to be crucial for semantics. -/
+@[reducible]
+def class_name (α : Type) [names α] :=
+  {name : α // name ∈ names.Nc α}
+@[reducible]
+def record_name (α : Type) [names α] :=
+  {name : α // name ∈ names.Nr α}
+@[reducible]
+def boolean_name (α : Type) [names α] : record_name α :=
+  ⟨names.Nboolean α, names.Hboolean α⟩
+@[reducible]
+def field_name [names α] (self : class_name α) :=
+  {name : α // name ∈ names.Nf self.property}
+@[reducible]
+def method_name [names α] (self : class_name α) :=
+  {name : α // name ∈ names.Nm self.property}
+@[reducible]
+def param_name [names α]
+    {self : class_name α} (m : method_name self) :=
+  {name : α // name ∈ names.Np m.property}
 
-  /- A class declaration (of some class self) consists of a map from field names to field declarations, a map from method names to method declarations, and a method name that indicates a constructor. A field declaration consists of a type. A method declaration consists of a map from parameter names to parameter declarations. A parameter declaration consists of a type. -/
-  variable {m : method_name self}
-  structure pdecl (p : param_name m) :=
-    (type : type α)
-  structure mdecl (m : method_name self) :=
-    (pdecl (p : param_name m) : pdecl p)
-  structure fdecl (f : field_name self) :=
-    (type : type α)
-  -- Design choice: constructors and methods are treated uniformly.
-  structure cdecl (self : class_name α) :=
-    (fdecl (f : field_name self) : fdecl f)
-    (mdecl (m : method_name self) : mdecl m)
-    (ctor : method_name self)
-end
-open type
+/- A type in our object language is either: a reference type (by class name), or a data type (by record name). -/
+@[derive decidable_eq]
+inductive type (α : Type) [names α]
+| ref: class_name α → type
+| data: record_name α → type
 
-/- A program signature consists of: a map from class names to class declarations, and a class name of the root object. -/
+/- A variable context is a list of types; a local variable is encoded by an index in this context. Local variables do not have a name. -/
+@[reducible] def context (α : Type) [names α] := list (type α)
+/- Boolean is a built-in data type. -/
+@[reducible] def boolean (α : Type) [names α] : type α :=
+  (type.data (boolean_name α))
+
+/- A class declaration (of some class self) consists of a map from field names to field declarations, a map from method names to method declarations, and a method name that indicates a constructor. A field declaration consists of a type. A method declaration consists of a map from parameter names to parameter declarations. A parameter declaration consists of a type. -/
+structure pdecl [names α]
+    {self : class_name α} {m : method_name self}
+    (p : param_name m) :=
+  (type : type α)
+structure mdecl [names α]
+    {self : class_name α} (m : method_name self) :=
+  (pdecl (p : param_name m) : pdecl p)
+structure fdecl [names α]
+    {self : class_name α} (f : field_name self) :=
+  (type : type α)
+-- Design choice: constructors and methods are treated uniformly.
+structure cdecl [names α] (self : class_name α) :=
+  (fdecl (f : field_name self) : fdecl f)
+  (mdecl (m : method_name self) : mdecl m)
+  (ctor : method_name self)
+  
+/- A record declaration is an inhabited type with decidable equality. -/
+structure rdecl :=
+  (host : Type)
+  (default: host)
+  (decidable_data: decidable_eq host)
+instance rdecl.to_sort : has_coe_to_sort rdecl :=
+  {S := Type, coe := λS, S.host}
+instance rdecl.host_decidable (γ : rdecl) :
+  decidable_eq γ := γ.decidable_data
+instance rdecl.host_inhabited (γ : rdecl) :
+  inhabited γ := ⟨γ.default⟩
+
+/- A signature consists of: a map from class names to class declarations, a map from record names to record declarations, and a class name of the root object. The built-in boolean is associated to a datatype equal to Lean's bool with false as default value, and we know Lean's bool is decidable. -/
 class signature (α : Type) extends names α : Type 1 :=
-(cdef (x : class_name α): cdecl x) (main: class_name α)
+  (cdef (x : class_name α): cdecl x)
+  (rdef (x : record_name α) : rdecl)
+  (main: class_name α)
+  (boolean_is_bool: (bool = (rdef (boolean_name α)).host))
+  (boolean_default_false: (rdef (boolean_name α)).default =
+    cast boolean_is_bool ff)
 
 variable [signature α]
 variable {self : class_name α}
@@ -79,15 +99,21 @@ def field_type (f : field_name self) : type α :=
   ((signature.cdef self).fdecl f).type
 def ctor (self : class_name α) : method_name self :=
   (signature.cdef self).ctor
-def class_type (self : class_name α) : type α :=
-  (ref self)
+def data_Type (r : record_name α) : Type :=
+  (signature.rdef r).host
+def data_default (r : record_name α) : data_Type r :=
+  (signature.rdef r).default
+lemma data_Type_eq_bool : bool = data_Type (boolean_name α) :=
+begin
+  unfold data_Type, apply signature.boolean_is_bool
+end
 
 /- Given a signature and an enclosing class, we consider type environments to consist of: a method name, and declared local variables. -/
+@[derive decidable_eq]
 structure tenv (self : class_name α) :=
   (current : method_name self)
   (locals : context α)
 def tenv.self (e : tenv self) : class_name α := self
-open tenv
 
 /- A note on terminology. Parameter: as declared in signature. Argument: a pure expression as supplied in a method call. -/
 
@@ -95,7 +121,7 @@ open tenv
 section
 variables (e : tenv self) (ty : type α)
 structure tvar :=
-  (H : ty = ref e.self)
+  (H : ty = type.ref e.self)
 structure lvar :=
   (idx : list_at ty e.locals)
 structure pvar :=
@@ -116,12 +142,12 @@ end
 
 /- A pure expression within a typing environment is either: a constant data value, a function application on data values, value lookup in environment, referential equality check. -/
 inductive pexp (e : tenv self) : type α → Type 1
-| const {γ : datatype}: γ → pexp (data α γ)
-| app {γ δ : datatype}: (γ.host → δ.host) →
-    pexp (data α γ) → pexp (data α δ)
+| const {r : record_name α}: data_Type r → pexp (type.data r)
+| app {r s : record_name α}: (data_Type r → data_Type s) →
+    pexp (type.data r) → pexp (type.data s)
 | lookup {ty : type α}: rvar e ty → pexp ty
 | requal {c : class_name α}:
-    pexp (ref c) → pexp (ref c) → pexp (boolean α)
+    pexp (type.ref c) → pexp (type.ref c) → pexp (boolean α)
 /- An argument list assigns to each parameter of a method a variable within some typing environment of the right type. -/
 structure arglist (e : tenv self)
     {c : class_name α} (m : method_name c) :=
@@ -135,10 +161,10 @@ inductive stmt (e : tenv self) : bool → Type 1
     pexp e ty → stmt ff
 | async (c : class_name α) (m : method_name c)
     (H : m ≠ ctor c)
-    (o : rvar e (ref c))
+    (o : rvar e (type.ref c))
     (τ : arglist e m): stmt ff
 | alloc (c : class_name α)
-    (l : svar e (ref c))
+    (l : svar e (type.ref c))
     (τ : arglist e (ctor c)): stmt ff
 | nil: stmt tt
 | cons: stmt ff → stmt tt → stmt tt
